Foundation/Propositional/FMT/Hilbert.lean
@@ -1,0 +1,74 @@
+import Foundation.Propositional.Hilbert.VF.Basic
+import Foundation.Propositional.FMT.Basic
+
+namespace LO.Propositional
+
+open FMT
+open Formula
+open Formula.FMT
+
+namespace Hilbert.VF.FMT
+
+variable {Ax Ax₁ Ax₂ : Axiom ℕ} {Γ : Set (Formula ℕ)} {φ : Formula ℕ}
+
+
+section FrameClass
+
+variable {C C₁ C₂ : FMT.FrameClass}
+
+lemma soundness_frameclass (hV : C ⊧* Ax) : (Hilbert.VF Ax) ⊢ φ → C ⊧ φ := by
+  intro hφ F hF;
+  induction hφ with
+  | axm hi => apply hV.models <;> assumption;
+  | _ => grind;
+
+instance instFrameClassSound (hV : C ⊧* Ax) : Sound (Hilbert.VF Ax) C := ⟨fun {_} => soundness_frameclass hV⟩
+
+lemma consistent_of_sound_frameclass (C : FMT.FrameClass) (hC : Set.Nonempty C) [sound : Sound (Hilbert.VF Ax) C] : Entailment.Consistent (Hilbert.VF Ax) := by
+  apply Entailment.Consistent.of_unprovable (φ := ⊥);
+  apply not_imp_not.mpr sound.sound;
+  apply Semantics.set_models_iff.not.mpr;
+  push_neg;
+  obtain ⟨F, hF⟩ := hC;
+  use F;
+  grind;
+
+lemma weakerThan_of_subset_frameClass (C₁ C₂ : FMT.FrameClass) (hC : C₂ ⊆ C₁) [Sound (Hilbert.VF Ax₁) C₁] [Complete (Hilbert.VF Ax₂) C₂] : (Hilbert.VF Ax₁) ⪯ (Hilbert.VF Ax₂) := by
+  apply Entailment.weakerThan_iff.mpr;
+  intro φ hφ;
+  apply Complete.complete (𝓜 := C₂);
+  intro F hF;
+  apply Sound.sound (𝓢 := (Hilbert.VF Ax₁)) (𝓜 := C₁) hφ;
+  apply hC hF;
+
+end FrameClass
+
+
+section ModelClass
+
+variable {C C₁ C₂ : FMT.ModelClass}
+
+lemma soundness_modelclass (hV : C ⊧* Ax) : (Hilbert.VF Ax) ⊢ φ → C ⊧ φ := by
+  intro hφ M hM;
+  induction hφ with
+  | axm hi => apply hV.models <;> assumption;
+  | _ => grind
+
+instance instModelClassSound (hV : C ⊧* Ax) : Sound (Hilbert.VF Ax) C := ⟨fun {_} => soundness_modelclass hV⟩
+
+lemma consistent_of_sound_modelclass (C : FMT.ModelClass) (hC : Set.Nonempty C) [sound : Sound (Hilbert.VF Ax) C] : Entailment.Consistent (Hilbert.VF Ax) := by
+  apply Entailment.Consistent.of_unprovable (φ := ⊥);
+  apply not_imp_not.mpr sound.sound;
+  apply Semantics.set_models_iff.not.mpr;
+  push_neg;
+  obtain ⟨M, hM⟩ := hC;
+  use M;
+  grind;
+
+end ModelClass
+
+
+end Hilbert.VF.FMT
+
+
+end LO.Propositional
