Foundation/Propositional/FMT/Logic/VF.lean
@@ -1,0 +1,96 @@
+import Foundation.Propositional.FMT.Hilbert
+import Foundation.Propositional.Hilbert.WF_VF
+
+
+namespace LO.Propositional
+
+open FMT
+
+
+namespace FMT
+
+protected abbrev FrameClass.VF : FMT.FrameClass := Set.univ
+
+abbrev trivialFrame : FMT.Frame where
+  World := Unit
+  Rel := λ _ _ _ => True
+  root := ()
+  rooted := by simp
+
+end FMT
+
+
+namespace VF
+
+open Hilbert.VF.FMT
+
+instance FMT.sound : Sound Propositional.VF FrameClass.VF := by
+  apply instFrameClassSound;
+  constructor;
+  tauto;
+
+
+open Formula.FMT
+
+instance : Entailment.Consistent Propositional.VF := consistent_of_sound_frameclass FrameClass.VF $ by
+  use FMT.trivialFrame;
+  apply Set.mem_setOf_eq.mpr;
+  simp;
+
+lemma unprovable_top_dntop : Propositional.VF ⊬ ⊤ ⭤ ∼∼⊤ := by
+  apply Sound.not_provable_of_countermodel (𝓜 := FMT.FrameClass.VF);
+  apply FMT.not_validOnFrameClass_of_exists_model_world;
+  let M : FMT.Model := {
+    World := Fin 3,
+    Rel φ x y :=
+      match φ with
+      | ⊤ ⭤ ∼∼⊤ => x ≤ y
+      | ∼∼⊤     => x ≤ y
+      | ∼⊤      => x ≠ 2
+      | _       => True
+    ,
+    root := 0,
+    rooted := by grind
+    Val _ _ := True
+  };
+  use M, 0
+  constructor;
+  . tauto;
+  . suffices ∃ x y : M, x ≺[∼⊤ ➝ ⊥] y ∧ ∀ (x : M), ¬y ≺[⊤ ➝ ⊥] x by simpa [M] using this;
+    use 1, 2;
+    grind;
+
+open Formula.FMT
+
+end VF
+
+open Formula.FMT in
+open Entailment.Corsi in
+instance : Propositional.VF ⪱ Propositional.WF := by
+  constructor;
+  . apply weakerThan_WF_VF_of_provable_axioms
+    simp [Entailment.ProvableSet]
+  . apply Entailment.not_weakerThan_iff.mpr;
+    use (⊤ ➝ #0 ⋏ #1) ⭤ (⊤ ➝ #1 ⋏ #0);
+    constructor;
+    . exact ruleE equivId $ andIR K_comm K_comm
+    . apply Sound.not_provable_of_countermodel (𝓜 := FMT.FrameClass.VF);
+      apply FMT.not_validOnFrameClass_of_exists_model_world;
+      use {
+        World := Fin 3,
+        Rel φ x y :=
+          match φ with
+          | ⊤ ➝ #1 ⋏ #0 => x ≤ y
+          | ⊤ ➝ #0 ⋏ #1 => x ≠ 1
+          | _       => True
+        ,
+        root := 0,
+        rooted := by grind
+        Val x a := x = 2 → a = 0
+      }, 0;
+      constructor;
+      . tauto;
+      . simp;
+        tauto;
+
+end LO.Propositional
